Shake build system working

build.hs
@@ -1,0 +1,13 @@
+#!/usr/bin/runhaskell
+
+import Development.Shake
+import Development.Shake.FilePath
+
+main = shakeArgs shakeOptions $ do  
+  want ["compiler.vo"]
+  "*.vo" %> \out -> do
+    let source = out -<.> ".v"
+    deps <- cmd $ "coqdep -I . " ++ source 
+    need $ drop 3 $ words $ fromStdout deps
+    cmd $ "coqc " ++ source
+  phony "clean" $ removeFilesAfter "." ["//*.vo", "//*.glob"]
