cesm.v
@@ -26,12 +26,12 @@ Notation " ⟨ Φ ⟩ m " := (conf Φ m) (at level 40).
 Notation " ⟨ Ψ , b ⟩ N " :=  (conf (cons b Ψ) N) (at level 40).
 Notation " ⟨ Φ , b , Ψ ⟩ N " := (conf (append _ Ψ (cons b Φ)) N) (at level 40).
 
-Fixpoint clu (v env:nat) (h:heap) : option nat := match v with
-  | 0 => Some env
-  | S n => match lookup eq_nat_dec env h with
-    | Some (cl c a) => clu n a h
+Fixpoint clu (v env:nat) (h:heap) : option (nat * closure) := match lookup eq_nat_dec env h with
+    | Some (cl c env') => match v with 
+      | 0 => Some (env, c) 
+      | S n => clu n env' h
+      end
     | None => None
-    end
   end.
 
 Definition fresh (n : nat) (h : heap) := 
@@ -73,30 +73,40 @@ Definition replaceClosure (l:nat) (c:closure) : nat * cell → nat * cell :=
     | (l', cl c' e) => if eq_nat_dec l l' then (l, cl c e) else x
     end.
 
-(*
-Definition step : {c1 | well_formed c1} → {c2 | well_formed c2}.
+(* Step as a function *
+
+Lemma well_formed_lookup : ∀ l h c e, well_formed_heap h → lookup eq_nat_dec l h = Some (cl c e) →
+  closed_under c h.
+intros l h c e wfh lu. 
+
+Lemma step : {c1 | well_formed c1} → {c2 | well_formed c2}.
 refine (
-  fun c1 => match c1 with
-  | exist (conf h s (close t e)) p => match t with
-    | var v => match clu v e h with
-      | Some l => match lookup eq_nat_dec l h with
-        | Some (cl c e') => exist well_formed (conf h (inr l::s) c) _
+  fun c1 => match c1 as Case1 return Case1 = c1 → {c2 | well_formed c2} with 
+  | exist c p => fun case1 => match c as Case2 return c = Case2 with 
+  | conf h s c' =>  match c' as Case2 return c' = with
+  | close t e => match t with
+    | var v => match clu v e h as Case4 return Case4 = clu v e h → {c2 | well_formed c2} with
+      | Some (l, _)  => λ case4, match lookup eq_nat_dec l h as Case5
+                        return Case5 = lookup eq_nat_dec l h → {c2 | well_formed c2} with
+        | Some (cl c e') => λ case5, exist well_formed (conf h (inr l::s) c) _
         | None => _
-        end
+      end eq_refl
       | None => _
-      end
+      end eq_refl
     | lam b => match s with
       | nil => c1
-      | cons (inl c) tl => let e' := new (proj1_sig c1) in 
-        exist well_formed (conf ((e', cl c e)::h) tl (close b e')) _
-      | cons (inr l) tl => exist well_formed 
-        (conf (map (replaceClosure l (close t e)) h) tl (close t e)) _
+      | cons (inl c) s' => let e' := new (proj1_sig c1) in 
+        exist well_formed (conf ((e', cl c e)::h) s' (close b e')) _
+      | cons (inr l) s' => exist well_formed 
+        (conf (map (replaceClosure l (close t e)) h) s' (close t e)) _
       end
     | app m n => exist well_formed (conf h (inl (close n e):: s) (close m e)) _
-    end
-  end
-).
-*)
+    end end end
+  end eq_refl
+). 
+unfold well_formed. split.   
 
+
+*)
 
 
