machine.v
@@ -1,0 +1,8 @@
+Require Import Unicode.Utf8.
+Require Import relations.
+
+Record machine (expr : Type) : Type := mkmachine {
+  state : Type;
+  insert : expr → state; 
+  step : transition state
+}.
