relations.v
@@ -1,0 +1,62 @@
+Require Import Unicode.Utf8. 
+
+Definition relation (X : Type) (Y : Type) := X → Y → Prop.
+
+Definition transition (X : Type) := X → X → Prop.
+
+Definition strong_bisim (A B : Type) (fa : transition A) (fb : transition B) (R : relation A B) :
+  Prop := ∀ a b, R a b → 
+          (∀ a', fa a a' → ∃ b', fb b b' ∧ R a' b')
+        ∧ (∀ b', fb b b' → ∃ a', fa a a' ∧ R a' b'). 
+
+Inductive refl_trans_clos {X} (f : transition X) : transition X := 
+  | t_refl (x : X) : refl_trans_clos f x x
+  | t_step (x y z : X) : f x y → refl_trans_clos f y z → refl_trans_clos f x z.
+
+(* p and q are bisimilar *)
+Notation "p '~' q" := (∃ fp fq R, strong_bisim p q fp fq R) (at level 30). 
+
+Definition partial_function {X Y: Type} (R: relation X Y) :=
+  ∀ (x : X) (y1 y2 : Y), R x y1 → R x y2 → y1 = y2. 
+
+Definition total_function {X Y: Type} (R: relation X Y) :=
+  (∀ x:X, ∃ y:Y, R x y) ∧ partial_function R. 
+
+Definition surjective {X Y: Type} (f : X → Y) : Prop :=
+  ∀ y:Y, ∃ x:X, f x = y.
+
+Definition injective {X Y : Type} (f : X → Y) : Prop :=
+  ∀ a b: X, f a = f b → a = b.
+
+Definition bijective {X Y : Type} (f : X → Y) : Prop :=
+  injective f ∧ surjective f.
+
+Definition reflexive {X : Type} (R: relation X X) :=
+  ∀ a : X, R a a.
+
+Definition symmetric {X : Type} (R: relation X X) :=
+  ∀ a b : X, (R a b) → (R b a).
+
+Definition antisymmetric {X: Type} (R: relation X X) :=
+  ∀ a b : X, (R a b) → (R b a) → a = b.
+
+Definition transitive {X: Type} (R: relation X X) :=
+  ∀ a b c : X, (R a b) → (R b c) → (R a c).
+
+Definition equivalence {X:Type} (R: relation X X) :=
+  (reflexive R) ∧ (symmetric R) ∧ (transitive R).
+
+Definition partial_order {X:Type} (R: relation X X) :=
+  (reflexive R) ∧ (antisymmetric R) ∧ (transitive R).
+
+(* Examples *)
+
+Inductive next_nat (n : nat) : nat → Prop := 
+    | succ : next_nat n (S n).
+
+(* simple bisimulation *)
+Theorem bisim_next_nat_eq : strong_bisim nat nat next_nat next_nat eq. 
+Proof. unfold strong_bisim. intros. subst. split. intros. apply ex_intro with a'.
+split; auto. intros. apply ex_intro with b'. split; auto. Qed. 
+
+
