README.md
@@ -1,0 +1,12 @@
+% Verifiably Lazy : A Verified Compiler for Call-By-Need.
+
+# Building / Proof Checking
+
+Requirements: 
+- `coqc` and `coqdep` (tested with 8.4)
+- `runhaskell` and Shake
+
+To Build: `./build.hs` (requires runhaskell and Shake, the Haskell build system) 
+
+
+
